investigations/acornish/AcornMonadDeep.v
@@ -1,0 +1,193 @@
+(****************************************************************************)
+(* Copyright 2021 The Project Oak Authors                                   *)
+(*                                                                          *)
+(* Licensed under the Apache License, Version 2.0 (the "License")           *)
+(* you may not use this file except in compliance with the License.         *)
+(* You may obtain a copy of the License at                                  *)
+(*                                                                          *)
+(*     http://www.apache.org/licenses/LICENSE-2.0                           *)
+(*                                                                          *)
+(* Unless required by applicable law or agreed to in writing, software      *)
+(* distributed under the License is distributed on an "AS IS" BASIS,        *)
+(* WITHOUT WARRANTIES OR CONDITIONS OF ANY KIND, either express or implied. *)
+(* See the License for the specific language governing permissions and      *)
+(* limitations under the License.                                           *)
+(****************************************************************************)
+
+(* Single monad structure, loop with fused delay *)
+
+Require Import Coq.Lists.List.
+Require Import Coq.ZArith.ZArith.
+Require Import ExtLib.Structures.Monad.
+Require Import ExtLib.Data.Monads.IdentityMonad.
+Require Import ExtLib.Data.List.
+
+Require Import Acornish.ListUtils.
+Require Import Acornish.Common.
+
+Require Import Cava.Util.List.
+
+Import ListNotations.
+Import MonadNotation.
+Local Open Scope monad_scope.
+Local Open Scope type_scope.
+
+Class Acorn acorn `{Monad acorn} (signal : SignalType -> Type) := {
+  inv : signal Bit -> acorn (signal Bit);
+  and2 : signal Bit * signal Bit -> acorn (signal Bit);
+  addMod : nat -> signal Nat * signal Nat -> acorn (signal Nat);
+  natDelay : signal Nat -> acorn (signal Nat);
+  (* loop : (signal Nat * signal Nat -> acorn (signal Nat * signal Nat)) -> *)
+  (*        signal Nat -> acorn (signal Nat); *)
+  constNat : nat -> acorn (signal Nat);
+  comparator : signal Nat * signal Nat -> acorn (signal Bit);
+  mux2 : signal Bit * (signal Nat * signal Nat) -> acorn (signal Nat);
+}.
+
+Inductive CavaDeep: SignalType -> Type :=
+| I : forall {a}, nat -> CavaDeep a
+
+| Inv : CavaDeep Bit -> CavaDeep Bit
+| And2 : CavaDeep Bit * CavaDeep Bit -> CavaDeep Bit
+| AddMod : nat -> CavaDeep Nat * CavaDeep Nat -> CavaDeep Nat
+| NatDelay : CavaDeep Nat -> CavaDeep Nat
+(* | Loop : (CavaDeep Nat * CavaDeep Nat -> ident (CavaDeep Nat * CavaDeep Nat)) -> *)
+(*          CavaDeep Nat -> CavaDeep Nat *)
+| ConstNat : nat -> CavaDeep Nat
+| Comparator : CavaDeep Nat * CavaDeep Nat -> CavaDeep Bit
+| Mux2 : CavaDeep Bit * (CavaDeep Nat * CavaDeep Nat) -> CavaDeep Nat.
+
+Instance AcornSimulation : Acorn ident CavaDeep := {
+  inv i := ret (Inv i);
+  and2 i := ret (And2 i);
+  addMod modBy i := ret (AddMod modBy i);
+  natDelay i := ret (NatDelay i);
+  (* loop s f i := fun '(s,s_inner) => *)
+  (*   let '(ns,(o,s')) := f (i,s) s_inner in *)
+  (*   (s',ns,o); *)
+  constNat n := ret (ConstNat n);
+  comparator i := ret (Comparator i);
+  mux2 i := ret (Mux2 i)
+}.
+
+Fixpoint state_shape {o} (c: CavaDeep o): list SignalType :=
+match c with
+| I _ => []
+| Inv x => state_shape x
+| And2 x => state_shape (fst x) ++ state_shape (snd x)
+| AddMod _ x => state_shape (fst x) ++ state_shape (snd x)
+| NatDelay x => state_shape x ++ [Nat]
+| ConstNat _ => []
+| Comparator x => state_shape (fst x) ++ state_shape (snd x)
+| Mux2 x => state_shape (fst x) ++ state_shape (fst (snd x)) ++ state_shape (snd (snd x))
+end.
+
+Definition get t1 t2 : denoteSignal t1 -> denoteSignal t2 :=
+  match t1 with
+  | Bit =>
+    match t2 with
+    | Bit => id
+    | _ => fun _=> resetVal _
+    end
+  | Nat =>
+    match t2 with
+    | Nat => id
+    | _ => fun _=> resetVal _
+    end
+  end.
+
+Definition input_map := nat -> {t&denoteSignal t}.
+
+Fixpoint step {o} (c: CavaDeep o) (input: input_map)
+  : denote_list denoteSignal (state_shape c) -> denote_list denoteSignal (state_shape c) * denoteSignal o :=
+match c with
+| @I x n => fun _ =>
+  let v := input n in
+  (tt, (get (projT1 v) x (projT2 v)))
+| Inv x => fun s =>
+  let (s', o) := step x input s in
+  (s', negb o)
+| And2 xy => fun s =>
+  let (sx,sy) := split_values s in
+  let (sx', x) := step (fst xy) input sx in
+  let (sy', y) := step (snd xy) input sy in
+  (combine_values sx' sy', andb x y)
+| AddMod modBy xy => fun s =>
+  let (sx,sy) := split_values s in
+  let (sx', x) := step (fst xy) input sx in
+  let (sy', y) := step (snd xy) input sy in
+  (combine_values sx' sy', (x+y) mod modBy)
+| NatDelay x => fun s =>
+  let (sx, so) := split_values s in
+  let (s', o) := step x input sx in
+  (combine_values (y:=[_]) s' (o,tt), fst so)
+| ConstNat n => fun s =>
+  (tt, n)
+| Comparator xy => fun s =>
+  let (sx,sy) := split_values s in
+  let (sx', x) := step (fst xy) input sx in
+  let (sy', y) := step (snd xy) input sy in
+  (combine_values sx' sy', y <=? x)
+| Mux2 ixy => fun s =>
+  let (si, sxy) := split_values s in
+  let (sx, sy) := split_values sxy in
+  let (si', i) := step (fst ixy) input si in
+  let (sx', x) := step (fst (snd ixy)) input sx in
+  let (sy', y) := step (snd (snd ixy)) input sy in
+  (combine_values si' (combine_values sx' sy'), if i then x else y)
+end.
+
+(* Run a circuit for many timesteps, starting at the reset value *)
+Definition simulate {o} (c : ident (CavaDeep o)) (input : list input_map) : list (denoteSignal o) :=
+  let c' := unIdent c in
+  fold_left_accumulate (fun i s => step c' s i) input (resetVals (state_shape c')).
+
+Section WithAcorn.
+  Context {acorn} {signal} `{Acorn acorn signal}.
+
+  (* Take a wire and fork it into two branches. *)
+  Definition fork2 {t : SignalType}
+              (a : signal t) : acorn (signal t * signal t) :=
+    ret (a, a).
+
+  (* Take a pair input and apply the circuit r to just the first element. *)
+  Definition fsT {t1 t2 t3 : SignalType}
+            (f : signal t1 -> acorn (signal t3))
+            (ab : signal t1 * signal t2) : acorn (signal t3 * signal t2) :=
+    let (a, b) := ab in
+    o <- f a ;;
+    ret (o, b).
+
+  (* Take a pair input and apply the circuit r to just the second element. *)
+  Definition snD {t1 t2 t3 : SignalType}
+            (f : signal t2 -> acorn (signal t3))
+            (ab : signal t1 * signal t2) : acorn (signal t1 * signal t3) :=
+    let (a, b) := ab in
+    o <- f b ;;
+    ret (a, o).
+
+  (* A circuit which delays the second element of a pair and then performs
+     a 256-bit addition of the two values in the pair. *)
+  Definition circuit1 : signal Nat * signal Nat -> acorn (signal Nat) :=
+    snD natDelay >=> addMod 256.
+
+  (* Definition counter6 : signal Nat -> acorn (signal Nat) := *)
+  (*   (1* loop (addMod 6 >=> natDelay >=> fork2). *1) *)
+  (*   loop (addMod 6 >=> fork2). *)
+
+  (* Definition nestedloop : signal Nat -> acorn _ (signal Nat) := *)
+  (*   loop (addMod 512 >=> loop (addMod 512 >=> fork2) >=> fork2). *)
+  (*   (1* loop (snD natDelay >=> addMod 512 >=> loop (addMod 512 >=> natDelay >=> fork2) >=> fork2). *1) *)
+
+End WithAcorn.
+
+(* We can easily simulate circuits without loops, even if they contain delay elements. *)
+Compute (simulate (circuit1 (I 0, I 1)) (
+  [ fun i => existT _ Nat (if Nat.eqb i 0 then 17 else 42)
+  ; fun i => existT _ Nat (if Nat.eqb i 0 then 78 else 62)
+  ; fun i => existT _ Nat (if Nat.eqb i 0 then 12 else 5)
+  ])).
+
+(*
+	 = [17; 120; 74]
+*)
