investigations/acornish/Common.v
@@ -1,0 +1,47 @@
+(****************************************************************************)
+(* Copyright 2021 The Project Oak Authors                                   *)
+(*                                                                          *)
+(* Licensed under the Apache License, Version 2.0 (the "License")           *)
+(* you may not use this file except in compliance with the License.         *)
+(* You may obtain a copy of the License at                                  *)
+(*                                                                          *)
+(*     http://www.apache.org/licenses/LICENSE-2.0                           *)
+(*                                                                          *)
+(* Unless required by applicable law or agreed to in writing, software      *)
+(* distributed under the License is distributed on an "AS IS" BASIS,        *)
+(* WITHOUT WARRANTIES OR CONDITIONS OF ANY KIND, either express or implied. *)
+(* See the License for the specific language governing permissions and      *)
+(* limitations under the License.                                           *)
+(****************************************************************************)
+
+Require Import Coq.Lists.List.
+Require Import Coq.ZArith.ZArith.
+
+Require Import Acornish.ListUtils.
+
+Import ListNotations.
+
+Inductive SignalType :=
+  | Bit : SignalType
+  | Nat : SignalType.
+
+Definition denoteSignal (t: SignalType) : Type :=
+  match t with
+  | Bit => bool
+  | Nat => nat
+  end.
+
+Definition resetVal (t: SignalType) : denoteSignal t :=
+  match t with
+  | Bit => false
+  | Nat => 0
+  end.
+
+Fixpoint resetVals (t: list SignalType) : denote_list denoteSignal t :=
+  match t with
+  | [] => tt
+  | x :: xs => (resetVal x, resetVals xs)
+  end.
+
+Definition split_values {x y} := split_denotation (x:=x) (y:=y) denoteSignal.
+Definition combine_values {x y} := combine_denotation (x:=x) (y:=y) denoteSignal.
